cleanup

complete-theory/compositionalityScript.sml
@@ -1,5 +1,5 @@
 
-open HolKernel boolLib bossLib Parse pred_setTheory boolTheory bagTheory
+open HolKernel boolLib bossLib Parse bagTheory listTheory
 val _ = new_theory "compositionality";
 
 val _ = add_rule
@@ -7,42 +7,35 @@ val _ = add_rule
   pp_elements = [TOK "(", TM, TOK ",", TM, TOK ")"], paren_style = OnlyIfNecessary,
   block_style = (AroundEachPhrase, (PP.INCONSISTENT, 2))};
 
-(*
 val _ = add_rule
   {term_name = "Assertional", fixity = Closefix,
   pp_elements = [TOK "Assertional(", TM, TOK ")"], paren_style = OnlyIfNecessary,
   block_style = (AroundEachPhrase, (PP.INCONSISTENT, 2))};
-*)
 
 val _ = add_rule {block_style = (AroundEachPhrase, (PP.INCONSISTENT, 2)),
-                  fixity = Infix(NONASSOC, 425),
-                  paren_style = OnlyIfNecessary,
-                  pp_elements = [TOK "-:"],
-                  term_name = "Implements"}
-
-val _ = add_rule {block_style = (AroundEachPhrase, (PP.INCONSISTENT, 2)),
-                  fixity = Infix(NONASSOC, 425),
+                  fixity = Infix(NONASSOC, 450),
                   paren_style = OnlyIfNecessary,
                   pp_elements = [TOK "◁"],
-                  term_name = "Implements"}
+                  term_name = "Impl"}
 
 val _ = add_rule {block_style = (AroundEachPhrase, (PP.INCONSISTENT, 2)),
-                  fixity = Infix(NONASSOC, 425),
+                  fixity = Infix(NONASSOC, 550),
                   paren_style = OnlyIfNecessary,
                   pp_elements = [TOK "⊑"],
                   term_name = "Refines"}
 
 val _ = add_rule {block_style = (AroundEachPhrase, (PP.INCONSISTENT, 2)),
-                  fixity = Infix(NONASSOC, 425),
+                  fixity = Infix(NONASSOC, 580),
                   paren_style = OnlyIfNecessary,
                   pp_elements = [TOK "⊓"],
                   term_name = "And"}
 
-val _ = add_rule {block_style = (AroundEachPhrase, (PP.INCONSISTENT, 2)),
-                  fixity = Infix(NONASSOC, 425),
+val _ = add_rule {block_style = (AroundEachPhrase, (PP.CONSISTENT, 0)),
+                  fixity = Infixl 581,
                   paren_style = OnlyIfNecessary,
                   pp_elements = [TOK "ₓ"],
                   term_name = "Composition"}
+
 
 Datatype:
   Term = Impl C S | Assertional S | Refines S S ;
@@ -57,102 +50,114 @@ End
 
 Definition S_M:
     (S_M (P α)             = {α})
-  ∧ (S_M (And s1 s2)       = (S_M s1) ∩ (S_M s2))
-  ∧ (S_M (Contract s1 s2)  = {b | ∀b'. C_M b' ∈ S_M s1 ⇒ C_M b' ∩ b ∈ S_M s2})
+  ∧ (S_M (s1 ⊓ s2)         = (S_M s1) ∩ (S_M s2))
+  ∧ (S_M (s1, s2)          = {b | ∀b'. C_M b' ∈ S_M s1 ⇒ C_M b' ∩ b ∈ S_M s2})
   ∧ (S_M (Parallell s1 s2) = {a ∩ b | a ∈ (S_M s1) ∧ b ∈ (S_M s2)})
 End
 
 Definition T_M:
-    (T_M (Impl c s)      ⇔ C_M c ∈ S_M s)
-  ∧ (T_M (Refines s1 s2) ⇔ S_M s1 ⊆ S_M s2)
+    (T_M (c ◁ s)      ⇔ C_M c ∈ S_M s)
+  ∧ (T_M (s1 ⊑ s2)     ⇔ S_M s1 ⊆ S_M s2)
 End
 
 Theorem IMPL_AX_THM:
-  ∀c s. T_M (Impl c s) ⇔ C_M c ∈ S_M s 
+  ∀c s. T_M (c ◁ s) ⇔ C_M c ∈ S_M s 
 Proof
   EVAL_TAC >>
   rw[]
 QED
 
 Theorem COMP_ASSOC_THM:
-  ∀c1 c2 c3 s. T_M (Impl (Composition (Composition c1 c2) c3) s) ⇔ T_M (Impl (Composition c1 (Composition c2 c3)) s)
+  ∀c1 c2 c3 s. T_M (c1 ₓ c2 ₓ c3 ◁ s) ⇔ T_M (c1 ₓ (c2 ₓ c3) ◁ s)
 Proof
   EVAL_TAC >>
   rw[] >>
   metis_tac[pred_setTheory.INTER_ASSOC]
 QED
 
+Theorem COMP_COMM_THM:
+  ∀c1 c2 s. T_M (c1 ₓ c2 ◁ s) ⇔ T_M (c2 ₓ c1 ◁ s)
+Proof
+  EVAL_TAC >>
+  rw[] >>
+  metis_tac[pred_setTheory.INTER_COMM]
+QED
+
 Theorem ELEM_IN_AND_THM:
-  ∀e s1 s2. e ∈ S_M s1 ∧ e ∈ S_M s2 ⇒ e ∈ S_M (And s1 s2)
+  ∀e s1 s2. e ∈ S_M s1 ∧ e ∈ S_M s2 ⇒ e ∈ S_M (s1 ⊓ s2)
 Proof
   EVAL_TAC >>
   rw[]
 QED
 
 Theorem AND_THM:
-  ∀c s1 s2. T_M (Impl c s1) ∧ T_M (Impl c s2) ⇒ T_M (Impl c (And s1 s2))
+  ∀c s1 s2. T_M (c ◁ s1) ∧ T_M (c ◁ s2) ⇒ T_M (c ◁ s1 ⊓ s2)
 Proof
   rw[] >>
   metis_tac[IMPL_AX_THM, ELEM_IN_AND_THM]
 QED
 
 Theorem AND_ELIM_1_THM:
-  ∀c s1 s2. T_M (Impl c (And s1 s2)) ⇒ T_M (Impl c s2)
+  ∀c s1 s2. T_M (c ◁ s1 ⊓ s2) ⇒ T_M (c ◁ s2)
 Proof
   EVAL_TAC >>
   rw[]
 QED
 
 Theorem AND_ELIM_2_THM:
-  ∀c s1 s2. T_M (Impl c (And s1 s2)) ⇒ T_M (Impl c s1)
+  ∀c s1 s2. T_M (c ◁ s1 ⊓ s2) ⇒ T_M (c ◁ s1)
 Proof
   EVAL_TAC >>
   rw[]
 QED
 
 Theorem REFINEMENT_THM:
-  ∀c s1 s2. T_M (Impl c s1) ∧ T_M (Refines s1 s2) ⇒ T_M (Impl c s2)
+  ∀c s1 s2. T_M (c ◁ s1) ∧ T_M (s1 ⊑ s2) ⇒ T_M (c ◁ s2)
 Proof
   EVAL_TAC >>
   metis_tac[pred_setTheory.SUBSET_DEF, pred_setTheory.SUBSET_TRANS]
 QED
 
 Theorem CONTRACT_ELIM_THM:
-  ∀c1 c2 s1 s2. T_M (Impl c1 s1) ∧ T_M(Impl c2 (s1, s2)) ⇒ T_M (Impl (Composition c1 c2) s2)
+  ∀c1 c2 s1 s2. T_M (c1 ◁ s1) ∧ T_M(c2 ◁ (s1, s2)) ⇒ T_M (c1 ₓ c2 ◁ s2)
 Proof
   EVAL_TAC >>
   rw[]
 QED
 
 Theorem SPEC_CONTRACT_INTRO_THM:
-  ∀c2 s1 s2. (∀q0. T_M (Impl q0 s1) ⇒ T_M (Impl (Composition q0 c2) s2)) ⇒ T_M (Impl c2 (s1,s2))
+  ∀c2 s1 s2. (∀q0. T_M (q0 ◁ s1) ⇒ T_M (q0 ₓ c2 ◁ s2)) ⇒ T_M (c2 ◁ (s1,s2))
 Proof
   EVAL_TAC >>
   rw[]
 QED
 
-(*
-define new and operator as part of term grammar
-*)
-
 Inductive G:
     (∀(t:α Term) Γ. (t <: Γ) ⇒ G Γ t) (* ax *)
   ∧ (∀t1 t2 Γ. G Γ t1 ∧ (T_M t1 ⇒ T_M t2) ⇒ G Γ t2) (* lower-level-imp *)
-  ∧ (∀q0 c s1 s2 Γ. G (BAG_INSERT (Impl q0 s1) Γ) (Impl (Composition q0 c) s2) ⇒ G Γ (Impl c (s1, s2))) (* contract *)
-  ∧ (∀c1 c2 s Γ. G Γ (Impl c1 s) ∧ BAG_IN (Assertional s) Γ ⇒ G Γ (Impl (Composition c1 c2) s)) 
+  ∧ (∀t1 t2 t3 Γ. G Γ t1 ∧ G Γ t2 ∧ (T_M t1 ∧ T_M t2 ⇒ T_M t3) ⇒ G Γ t3) (* lower-level-imp *)
+  ∧ (∀q0 c s1 s2 Γ. G (BAG_INSERT (q0 ◁ s1) Γ) ((q0 ₓ c) ◁ s2) ⇒ G Γ (c ◁ (s1, s2))) (* contract *)
+  ∧ (∀c1 c2 s Γ. G Γ (c1 ◁ s) ∧ BAG_IN (Assertional s) Γ ⇒ G Γ (c1 ₓ c2 ◁ s)) 
   ∧ (∀t1 t2 Γ . G Γ t1 ⇒ G (BAG_INSERT t2 Γ) t1) (* closure *)
 End
 
-val [G_AX, G_LOWER_IMP, G_CONTRACT_AX, G_ASSERTION, G_CLOSURE] = CONJUNCTS G_rules;
+val [G_AX, G_LOWER_IMP, G_LOWER_IMP2, G_CONTRACT_AX, G_ASSERTION, G_CLOSURE] = CONJUNCTS G_rules;
 
 Theorem G_REFINEMENT_THM:
-  ∀c s1 s2 Γ. G Γ ((Impl c s1)) ∧ (BAG_IN (Refines s1 s2) Γ) ⇒ G Γ (Impl c s2)
+  ∀c s1 s2 Γ. G Γ (c ◁ s1) ∧ (BAG_IN (s1 ⊑ s2) Γ) ⇒ G Γ (c ◁ s2)
 Proof
   rw[] >>
-  ‘G Γ (Refines s1 s2)’ by metis_tac[G_AX] >>
+  ‘G Γ (s1 ⊑ s2)’ by metis_tac[G_AX] >>
   ASSUME_TAC REFINEMENT_THM >>
   metis_tac[G_LOWER_IMP] >>
   metis_tac[G_AX, REFINEMENT_THM, G_LOWER_IMP]
+QED
+
+Theorem G_CONTRACT_ELIM_THM:
+  ∀c1 c2 s1 s2 Γ. G Γ (c1 ◁ s1) ∧ G Γ (c2 ◁ (s1, s2)) ⇒ G Γ (c1 ₓ c2 ◁ s2)
+Proof
+  rw[] >>
+  metis_tac[G_LOWER_IMP, CONTRACT_ELIM_THM]
 QED
 
 (*
@@ -175,28 +180,46 @@ val comp_rules = [ELEM_IN_AND_THM,
                   REFINEMENT_THM,
                   G_AX,
                   G_LOWER_IMP,
+                  G_LOWER_IMP2,
                   G_CONTRACT_AX,
                   G_ASSERTION,
                   G_REFINEMENT_THM,
+                  G_CONTRACT_ELIM_THM,
                   G_CLOSURE,
                   BAG_IN_BAG_INSERT,
-                  COMP_ASSOC_THM];
-
-
+                  COMP_ASSOC_THM,
+                  COMP_COMM_THM];
 (*
 Context menu
 
 Pallet
 *)
 
-Theorem TEST:
+Definition COMPOSITIONALITY_TAC:
+  COMPOSITIONALITY_TAC = metis_tac comp_rules
+End
+
+Theorem PAPER_EXAMPLE:
   let
-    Γ = {|Assertional a; Refines a a1; Refines (And a g1) a2; Refines g2 g|}
+    Γ = {|Assertional a; a ⊑ a1; (a ⊓ g1) ⊑ a2; g2 ⊑ g|}
   in
-    G Γ (Impl c1 (a1, g1)) ∧ G Γ (Impl c2 (a2, g2)) ⇒ G Γ (Impl (Composition c1 c2) (a, g))
+    G Γ (c1 ◁ (a1, g1)) ∧ G Γ (c2 ◁ (a2, g2)) ⇒ G Γ (c1 ₓ c2 ◁ (a, g))
 Proof
   rw[] >>
-  ‘G {|Assertional a; Refines a a1; Refines (And a g1) a2; Refines g2 g|} (Impl (Composition c1 c2) (a, g))’ by metis_tac comp_rules
+  metis_tac comp_rules
+QED
+
+Theorem FUEL_LEVEL_DISPLAY_CONTROLLER:
+    Γ = {|g_I ⊑ a_A;
+          g_ADC ⊑ a_I; g_A ⊑ a_DAC;
+          g_T ⊑ a_ADC; g_DAC ⊑ a_D;|}
+    ∧ G Γ (c_I ◁ (a_I, g_I)) ∧ G Γ (c_A ◁ (a_A, g_A)) (* Program components *)
+    ∧ G Γ (c_ADC ◁ (a_ADC, g_ADC)) ∧ G Γ (c_DAC ◁ (a_DAC, g_DAC)) (* Controller components *)
+    ∧ G Γ (c_T ◁ (a_T, g_T)) ∧ G Γ (c_D ◁ (a_D, g_D)) (* Additional system components *)
+  ⇒ G Γ ((c_T ₓ c_ADC ₓ c_I ₓ c_A ₓ c_DAC ₓ c_D) ◁ (a_T, g_D))
+Proof
+  rw[] >>
+  metis_tac comp_rules
 QED
 
 val _ = export_theory();
