README.md
@@ -1,2 +1,8 @@
 # Compositionality Theory in HOL4
 This repository contains two formalizations of a compositionality theory for the theorem prover [HOL4](https://hol-theorem-prover.org).
+
+### Shortkeys for inserting
+C-S-M-q q - ⊑
+C-S-M-q i - ⊓
+C-M-_ x - ₓ
+C-M-| , - ◁
